Checkpoint an attempt at commit'ing a non-deterministic state.
Naive approach to specify non-determinism: in the post-condition of the
function (which we're about to wrap in a transaction), assert that the
resulting mem is just some mem that satisfies some externally-supplied
predicate.

This approach fails, for a somewhat surprising reason:

The post-condition in question gets copied in several places during
the proof (perhaps by spost, perhaps by the hoare tactic, perhaps by
something else).  There's nothing that requires the different copies
of this post-condition to produce the same mem; only that all of them
satisfy the externally-supplied predicate.  As a result, the proof gets
stuck with two possibly-different mem's satisfying the same predicate.

src/HoareLogicN.v
@@ -1047,9 +1047,9 @@ Definition wrappable (R:Set) (p:prog R) (fn:mem->mem) := forall m0 m,
   {{r, Log.rep the_xp (ActiveTxn (m0, fn m))
     \/ ([r = Crashed] /\ exists m', Log.rep the_xp (ActiveTxn (m0, m')))}}.
 
-Definition txn_wrap (p:prog unit) (fn:mem->mem) (wrappable_p: wrappable p fn) := $(mem:
+Definition txn_wrap (p:prog unit) (fn:mem->mem) (wr: wrappable p fn) := $(unit:
   Call1 (Log.begin_ok the_xp);;
-  Call2 (wrappable_p);;
+  Call2 (wr);;
   Call2 (Log.commit_ok the_xp)
 ).
 
@@ -1193,3 +1193,52 @@ Parameter A2OK: DataStart the_xp <= a2 < DataStart the_xp + DataLen the_xp.
 Check (txn_wrap (write_two_blocks_wrappable v1 v2 A1OK A2OK)).
 Check (txn_wrap_ok (write_two_blocks_wrappable v1 v2 A1OK A2OK)).
 
+
+
+Definition wrappable_nd (R:Set) (p:prog R) (ok:pred) := forall m,
+  {{Log.rep the_xp (ActiveTxn (m, m))}}
+  p
+  {{r, (exists m', Log.rep the_xp (ActiveTxn (m, m')) /\ [ok m'])
+    \/ ([r = Crashed] /\ exists m', Log.rep the_xp (ActiveTxn (m, m')))}}.
+
+Definition txn_wrap_nd (p:prog unit) (ok:pred) (wr: wrappable_nd p ok) := $(unit:
+  Call1 (Log.begin_ok the_xp);;
+  Call1 (wr);;
+  Call2 (Log.commit_ok the_xp)
+).
+
+Theorem txn_wrap_nd_ok_norecover:
+  forall (p:prog unit) (ok:pred) (wr: wrappable_nd p ok) m,
+  {{Log.rep the_xp (NoTransaction m)}}
+  (txn_wrap_nd wr)
+  {{r, (exists m', Log.rep the_xp (NoTransaction m') /\ [ok m'])
+    \/ ([r = Crashed] /\ (Log.rep the_xp (NoTransaction m) \/
+                          (exists m', Log.rep the_xp (ActiveTxn (m, m'))) \/
+                          (exists m', Log.rep the_xp (CommittedTxn m') /\ [ok m'])))}}.
+Proof.
+  hoare.
+  - destruct (H0 m); clear H0; pred.
+  - destruct (H1 m); clear H1; pred.
+    destruct (H0 m); clear H0; pred.
+    destruct (H1 m); clear H1; pred.
+  - destruct (H2 m); clear H2; pred.
+    destruct (H1 m); clear H1; pred.
+    + destruct (H2 m); clear H2; pred.
+    + (* we have our non-deterministic mem: x4 *)
+      destruct (H0 m x4); clear H0; pred.
+
+      destruct (H5 m); clear H5; pred.
+      destruct (H1 m); clear H1; pred.
+      destruct (H5 m); clear H5; pred.
+      (* XXX so close but something is broken..
+       * we need to prove:
+       *   Log.rep the_xp (ActiveTxn (m, x4)) m1
+       * but we have:
+       *   Log.rep the_xp (ActiveTxn (m, x7)) m1
+       * where x7 and x4 are two possibly-different mem's, both of which satisfy ok.
+       *
+       * seems like the pre-/post-conditions of wr get copied to several places,
+       * and when we destruct them, we end up with two possibly-different mem's,
+       * since there's no constraint that they be the same..
+       *)
+Aborted.
